proof/invariants/IWritePhysical.v
@@ -2675,20 +2675,23 @@ Qed.
 Lemma insertEntryIntoLLPCUpdateLLCouplePPVA s ptMMUTrdVA phySh2addr phySh1addr indMMUToPrepare ptMMUFstVA phyMMUaddr lastLLTable
       phyPDChild currentShadow2 phySh2Child currentPD ptSh1TrdVA ptMMUSndVA ptSh1SndVA ptSh1FstVA currentShadow1
       descChildphy phySh1Child currentPart trdVA nextVA vaToPrepare sndVA fstVA nbLgen l idxFstVA idxSndVA idxTrdVA
-      zeroI lpred newLastLLable nextFFI (* (LLDescChild:page) *) entry fstLL LLChildphy:
+      zeroI lpred newLastLLable nextFFI (* (LLDescChild:page) *) entry fstLL LLChildphy pgvalue minFI FFI:
+isIndexValue newLastLLable (CIndex 0) FFI s ->
+StateLib.Index.succ FFI = Some nextFFI ->      
 lookup newLastLLable nextFFI (memory s) beqPage beqIndex = Some (I entry) ->
 StateLib.getMaxIndex <> Some nextFFI ->  
 insertEntryIntoLLPC s ptMMUTrdVA phySh2addr phySh1addr indMMUToPrepare ptMMUFstVA phyMMUaddr lastLLTable
       phyPDChild currentShadow2 phySh2Child currentPD ptSh1TrdVA ptMMUSndVA ptSh1SndVA ptSh1FstVA currentShadow1
       descChildphy phySh1Child currentPart trdVA nextVA vaToPrepare sndVA fstVA nbLgen l idxFstVA idxSndVA idxTrdVA
-      zeroI lpred fstLL LLChildphy newLastLLable ->
+      zeroI lpred fstLL LLChildphy newLastLLable minFI ->
 insertEntryIntoLLPC {|
   currentPartition := currentPartition s;
-  memory := add newLastLLable nextFFI (PP phyMMUaddr) (memory s) beqPage beqIndex |} ptMMUTrdVA phySh2addr phySh1addr indMMUToPrepare ptMMUFstVA phyMMUaddr lastLLTable
+  memory := add newLastLLable nextFFI (PP pgvalue) (memory s) beqPage beqIndex |} ptMMUTrdVA phySh2addr phySh1addr indMMUToPrepare ptMMUFstVA phyMMUaddr lastLLTable
       phyPDChild currentShadow2 phySh2Child currentPD ptSh1TrdVA ptMMUSndVA ptSh1SndVA ptSh1FstVA currentShadow1
       descChildphy phySh1Child currentPart trdVA nextVA vaToPrepare sndVA fstVA nbLgen l idxFstVA idxSndVA idxTrdVA
-      zeroI lpred fstLL LLChildphy newLastLLable.
+      zeroI lpred fstLL LLChildphy newLastLLable minFI.
 Proof.
+intros HFFI HnextFFI.
 intros Hlookup Hkey2.
 intros.
 set(s':=  {|
@@ -2769,6 +2772,10 @@ unfold insertEntryIntoLLPC, propagatedPropertiesPrepare in *;intuition;subst;sim
   symmetry.
   apply getLLPagesUpdateLLCouplePPVA;trivial.
   rewrite <- Hconf;trivial.
++ assert(exists NbFI : index, isIndexValue newLastLLable (CIndex 1) NbFI s /\ NbFI >= CIndex minFI) as (x & Hx & Hx1) by trivial.
+  exists x;split;trivial.
+  apply isIndexValueUpdateLLCouplePPVA;trivial. right.
+admit. (** consistency property not found:  LLconfiguration5' (CIndex 1 <> nextFFI*) 
 + unfold writeAccessibleRecPreparePostconditionAll in *;intuition;
   apply writeAccessibleRecPreparePostconditionUpdateLLCouplePPVA with entry;trivial.
 + unfold isWellFormedTables in *; intuition.
@@ -2778,7 +2785,7 @@ unfold insertEntryIntoLLPC, propagatedPropertiesPrepare in *;intuition;subst;sim
 + apply isEntryVAUpdateLLCouplePPVA with entry;trivial.
 + apply isEntryVAUpdateLLCouplePPVA with entry;trivial.
 + apply isEntryVAUpdateLLCouplePPVA with entry;trivial.  
-Qed.
+Admitted.
 
 Lemma isPP'SameValueUpdateLLCouplePPVA  newLastLLable nextFFI phyMMUaddr s:
 isPP' newLastLLable nextFFI phyMMUaddr
