proof/invariants/InitFstShadow.v
@@ -300,12 +300,12 @@ Qed.
 
 Lemma initFstShadowPrepareHT lpred ptMMUTrdVA phySh2addr phySh1addr indMMUToPrepare ptMMUFstVA phyMMUaddr
       lastLLTable phyPDChild currentShadow2 phySh2Child currentPD ptSh1TrdVA ptMMUSndVA ptSh1SndVA ptSh1FstVA
-      currentShadow1 descChildphy phySh1Child currentPart trdVA nextVA vaToPrepare sndVA fstVA nbLgen l  idxFstVA idxSndVA idxTrdVA zeroI LLroot LLChildphy newLastLLable:
+      currentShadow1 descChildphy phySh1Child currentPart trdVA nextVA vaToPrepare sndVA fstVA nbLgen l  idxFstVA idxSndVA idxTrdVA zeroI LLroot LLChildphy newLastLLable minFI:
 {{ fun s : state =>
 (propagatedPropertiesPrepare LLroot LLChildphy newLastLLable s ptMMUTrdVA phySh2addr phySh1addr indMMUToPrepare ptMMUFstVA phyMMUaddr
   lastLLTable phyPDChild currentShadow2 phySh2Child currentPD ptSh1TrdVA ptMMUSndVA ptSh1SndVA ptSh1FstVA
   currentShadow1 descChildphy phySh1Child currentPart trdVA nextVA vaToPrepare sndVA fstVA nbLgen l false
-  false false true true true idxFstVA idxSndVA idxTrdVA zeroI 
+  false false true true true idxFstVA idxSndVA idxTrdVA zeroI minFI
 /\ isPartitionFalseAll s ptSh1FstVA ptSh1TrdVA ptSh1SndVA idxFstVA idxSndVA idxTrdVA 
 /\ writeAccessibleRecPreparePostcondition currentPart phyMMUaddr s 
 /\ writeAccessibleRecPreparePostcondition currentPart phySh1addr s 
@@ -315,7 +315,7 @@ Lemma initFstShadowPrepareHT lpred ptMMUTrdVA phySh2addr phySh1addr indMMUToPrep
 {{fun _ s => (propagatedPropertiesPrepare LLroot LLChildphy newLastLLable s ptMMUTrdVA phySh2addr phySh1addr indMMUToPrepare ptMMUFstVA phyMMUaddr
   lastLLTable phyPDChild currentShadow2 phySh2Child currentPD ptSh1TrdVA ptMMUSndVA ptSh1SndVA ptSh1FstVA
   currentShadow1 descChildphy phySh1Child currentPart trdVA nextVA vaToPrepare sndVA fstVA nbLgen l false
-  false false true true true idxFstVA idxSndVA idxTrdVA zeroI 
+  false false true true true idxFstVA idxSndVA idxTrdVA zeroI minFI
 /\ isPartitionFalseAll s ptSh1FstVA ptSh1TrdVA ptSh1SndVA idxFstVA idxSndVA idxTrdVA 
 /\ writeAccessibleRecPreparePostcondition currentPart phyMMUaddr s
 /\ writeAccessibleRecPreparePostcondition currentPart phySh1addr s
