proof/invariants/InitPEntryTable.v
@@ -1813,12 +1813,12 @@ Qed.
 
  Lemma initPEntryTablePropagateProperties curidx table ptMMUTrdVA phySh2addr phySh1addr indMMUToPrepare ptMMUFstVA phyMMUaddr lastLLTable phyPDChild
         currentShadow2 phySh2Child currentPD ptSh1TrdVA ptMMUSndVA ptSh1SndVA ptSh1FstVA currentShadow1 descChildphy phySh1Child
-        currentPart trdVA nextVA vaToPrepare sndVA fstVA nbLgen l idxFstVA idxSndVA idxTrdVA lpred zeroI LLroot LLChildphy newLastLLable:
+        currentPart trdVA nextVA vaToPrepare sndVA fstVA nbLgen l idxFstVA idxSndVA idxTrdVA lpred zeroI LLroot LLChildphy newLastLLable minFI:
 {{ fun s : state =>
 propagatedPropertiesPrepare LLroot LLChildphy newLastLLable s ptMMUTrdVA phySh2addr phySh1addr indMMUToPrepare ptMMUFstVA phyMMUaddr
         lastLLTable phyPDChild currentShadow2 phySh2Child currentPD ptSh1TrdVA ptMMUSndVA ptSh1SndVA ptSh1FstVA
         currentShadow1 descChildphy phySh1Child currentPart trdVA nextVA vaToPrepare sndVA fstVA nbLgen l false
-        false false true true true idxFstVA idxSndVA idxTrdVA zeroI
+        false false true true true idxFstVA idxSndVA idxTrdVA zeroI minFI
 /\ isPartitionFalseAll s ptSh1FstVA ptSh1TrdVA ptSh1SndVA idxFstVA idxSndVA idxTrdVA
 /\ writeAccessibleRecPreparePostcondition currentPart phyMMUaddr s 
 /\ writeAccessibleRecPreparePostcondition currentPart phySh1addr s 
@@ -1832,7 +1832,7 @@ propagatedPropertiesPrepare LLroot LLChildphy newLastLLable s ptMMUTrdVA phySh2a
 {{ fun _ (s : state) => propagatedPropertiesPrepare LLroot LLChildphy newLastLLable s ptMMUTrdVA phySh2addr phySh1addr indMMUToPrepare ptMMUFstVA phyMMUaddr
         lastLLTable phyPDChild currentShadow2 phySh2Child currentPD ptSh1TrdVA ptMMUSndVA ptSh1SndVA ptSh1FstVA
         currentShadow1 descChildphy phySh1Child currentPart trdVA nextVA vaToPrepare sndVA fstVA nbLgen l false
-        false false true true true idxFstVA idxSndVA idxTrdVA zeroI
+        false false true true true idxFstVA idxSndVA idxTrdVA zeroI minFI
 /\ isPartitionFalseAll s ptSh1FstVA ptSh1TrdVA ptSh1SndVA idxFstVA idxSndVA idxTrdVA 
 /\ writeAccessibleRecPreparePostcondition currentPart phyMMUaddr s 
 /\ writeAccessibleRecPreparePostcondition currentPart phySh1addr s 
