proof/invariants/UpdateMappedPageContent.v
@@ -5883,7 +5883,7 @@ apply Hcond;trivial.
 Qed.
 Lemma  propagatePropertiesPrepareUpdateMappedPageContent  s table curidx ptMMUTrdVA phySh2addr phySh1addr indMMUToPrepare ptMMUFstVA phyMMUaddr lastLLTable phyPDChild
             currentShadow2 phySh2Child currentPD ptSh1TrdVA ptMMUSndVA ptSh1SndVA ptSh1FstVA currentShadow1 descChildphy phySh1Child
-            currentPart trdVA nextVA vaToPrepare sndVA fstVA nbLgen l idxFstVA idxSndVA idxTrdVA x zeroI fstLL LLChildphy newLastLLable:
+            currentPart trdVA nextVA vaToPrepare sndVA fstVA nbLgen l idxFstVA idxSndVA idxTrdVA x zeroI fstLL LLChildphy newLastLLable n:
 match x with 
 | PE a => isPresentNotDefaultIff {|
                     currentPartition := currentPartition s;
@@ -5893,7 +5893,7 @@ match x with
 end ->             
  propagatedPropertiesPrepare fstLL LLChildphy newLastLLable s ptMMUTrdVA phySh2addr phySh1addr indMMUToPrepare ptMMUFstVA phyMMUaddr lastLLTable phyPDChild
             currentShadow2 phySh2Child currentPD ptSh1TrdVA ptMMUSndVA ptSh1SndVA ptSh1FstVA currentShadow1 descChildphy phySh1Child
-            currentPart trdVA nextVA vaToPrepare sndVA fstVA nbLgen l false false false true true true idxFstVA idxSndVA idxTrdVA zeroI -> 
+            currentPart trdVA nextVA vaToPrepare sndVA fstVA nbLgen l false false false true true true idxFstVA idxSndVA idxTrdVA zeroI n -> 
  initPEntryTablePreconditionToPropagatePrepareProperties s table -> 
  propagatedPropertiesPrepare fstLL LLChildphy newLastLLable
    {|      currentPartition := currentPartition s;
@@ -5902,7 +5902,7 @@ end ->
   phySh2addr phySh1addr indMMUToPrepare ptMMUFstVA phyMMUaddr lastLLTable phyPDChild
   currentShadow2 phySh2Child currentPD ptSh1TrdVA ptMMUSndVA ptSh1SndVA ptSh1FstVA
   currentShadow1 descChildphy phySh1Child currentPart trdVA nextVA vaToPrepare sndVA
-  fstVA nbLgen l false false false true true true idxFstVA idxSndVA idxTrdVA zeroI.
+  fstVA nbLgen l false false false true true true idxFstVA idxSndVA idxTrdVA zeroI n.
 Proof.
 intros.
 set (s' := {|
